add AReturns and EReturns, factor out the Q from eq_sat_sep_sbuter

src/Temporal_new.v
@@ -47,9 +47,9 @@ Hint Resolve sbuter_gen_mon : paco.
 Definition TPred S R := CompM S R -> S -> Prop.
 Definition TPred' S R := CompM' S R -> S -> Prop.
 
-Definition eq_sat_sep_sbuter {S1 S2 R1 R2} (q:@perm (S1*S2))
+Definition eq_sat_sep_sbuter {S1 S2 R1 R2} (q:@perm (S1*S2)) Q
   (P1:TPred S1 R1) (P2:TPred S2 R2) :=
-  forall p Q t1 s1 t2 s2, pre q (s1,s2) -> p ⊥ q ->
+  forall p t1 s1 t2 s2, pre q (s1,s2) -> p ⊥ q ->
     sbuter p Q t1 s1 t2 s2 -> no_errors t2 s2 ->
     (P1 t1 s1 <-> P2 t2 s2).
 Hint Unfold eq_sat_sep_sbuter : core.
@@ -62,31 +62,31 @@ Definition state_pred {S} R P : TPred S R := fun '_ s => P s.
 Definition q_similar {S1 S2} q (P1 : S1 -> Prop) (P2 : S2 -> Prop): Prop :=
   forall s1 s2, pre q (s1,s2) -> (P1 s1 <-> P2 s2).
 
-Lemma eq_sat_state_preds {S1 S2 R1 R2} q (P1 : S1 -> Prop) (P2 : S2 -> Prop)
+Lemma eq_sat_state_preds {S1 S2 R1 R2} q Q (P1 : S1 -> Prop) (P2 : S2 -> Prop)
   : q_similar q P1 P2 ->
-    eq_sat_sep_sbuter q (state_pred R1 P1) (state_pred R2 P2).
+    eq_sat_sep_sbuter q Q (state_pred R1 P1) (state_pred R2 P2).
 Proof. intros; eauto. Qed.
 
 
 (** * `eq_sat_sep_sbuter` for logical connectives **)
 
-Lemma eq_sat_and {S1 S2 R1 R2} q (TP1 TP1' : TPred S1 R1) (TP2 TP2' : TPred S2 R2)
-  : eq_sat_sep_sbuter q TP1 TP2 -> eq_sat_sep_sbuter q TP1' TP2' ->
-    eq_sat_sep_sbuter q (TP1 /2\ TP1') (TP2 /2\ TP2').
+Lemma eq_sat_and {S1 S2 R1 R2} q Q (TP1 TP1' : TPred S1 R1) (TP2 TP2' : TPred S2 R2)
+  : eq_sat_sep_sbuter q Q TP1 TP2 -> eq_sat_sep_sbuter q Q TP1' TP2' ->
+    eq_sat_sep_sbuter q Q (TP1 /2\ TP1') (TP2 /2\ TP2').
 Proof.
-  intros esss esss' p Q t1 s1 t2 s2 pre_q sep sb no_errs.
-  rewrite (esss p Q t1 s1 t2 s2 pre_q sep sb no_errs).
-  rewrite (esss' p Q t1 s1 t2 s2 pre_q sep sb no_errs).
+  intros esss esss' p t1 s1 t2 s2 pre_q sep sb no_errs.
+  rewrite (esss p t1 s1 t2 s2 pre_q sep sb no_errs).
+  rewrite (esss' p t1 s1 t2 s2 pre_q sep sb no_errs).
   reflexivity.
 Qed.
 
-Lemma eq_sat_or {S1 S2 R1 R2} q (TP1 TP1' : TPred S1 R1) (TP2 TP2' : TPred S2 R2)
-  : eq_sat_sep_sbuter q TP1 TP2 -> eq_sat_sep_sbuter q TP1' TP2' ->
-    eq_sat_sep_sbuter q (TP1 \2/ TP1') (TP2 \2/ TP2').
+Lemma eq_sat_or {S1 S2 R1 R2} q Q (TP1 TP1' : TPred S1 R1) (TP2 TP2' : TPred S2 R2)
+  : eq_sat_sep_sbuter q Q TP1 TP2 -> eq_sat_sep_sbuter q Q TP1' TP2' ->
+    eq_sat_sep_sbuter q Q (TP1 \2/ TP1') (TP2 \2/ TP2').
 Proof.
-  intros esss esss' p Q t1 s1 t2 s2 pre_q sep sb no_errs.
-  rewrite (esss p Q t1 s1 t2 s2 pre_q sep sb no_errs).
-  rewrite (esss' p Q t1 s1 t2 s2 pre_q sep sb no_errs).
+  intros esss esss' p t1 s1 t2 s2 pre_q sep sb no_errs.
+  rewrite (esss p t1 s1 t2 s2 pre_q sep sb no_errs).
+  rewrite (esss' p t1 s1 t2 s2 pre_q sep sb no_errs).
   reflexivity.
 Qed.
 
@@ -94,13 +94,13 @@ Notation "p -2> q" :=
   (fun x0 x1 => p x0 x1 -> q x0 x1)
   (at level 50, no associativity).
 
-Lemma eq_sat_impl {S1 S2 R1 R2} q (TP1 TP1' : TPred S1 R1) (TP2 TP2' : TPred S2 R2)
-  : eq_sat_sep_sbuter q TP1 TP2 -> eq_sat_sep_sbuter q TP1' TP2' ->
-    eq_sat_sep_sbuter q (TP1 -2> TP1') (TP2 -2> TP2').
+Lemma eq_sat_impl {S1 S2 R1 R2} q Q (TP1 TP1' : TPred S1 R1) (TP2 TP2' : TPred S2 R2)
+  : eq_sat_sep_sbuter q Q TP1 TP2 -> eq_sat_sep_sbuter q Q TP1' TP2' ->
+    eq_sat_sep_sbuter q Q (TP1 -2> TP1') (TP2 -2> TP2').
 Proof.
-  intros esss esss' p Q t1 s1 t2 s2 pre_q sep sb no_errs.
-  rewrite (esss p Q t1 s1 t2 s2 pre_q sep sb no_errs).
-  rewrite (esss' p Q t1 s1 t2 s2 pre_q sep sb no_errs).
+  intros esss esss' p t1 s1 t2 s2 pre_q sep sb no_errs.
+  rewrite (esss p t1 s1 t2 s2 pre_q sep sb no_errs).
+  rewrite (esss' p t1 s1 t2 s2 pre_q sep sb no_errs).
   reflexivity.
 Qed.
 
@@ -109,11 +109,13 @@ Qed.
 
 Inductive EU {S R} (P P' : TPred S R) t0 s0 : Prop :=
 | EU_here : P' t0 s0 -> EU P P' t0 s0
-| EU_step t1 s1 : P t0 s0 -> step t0 s0 t1 s1 -> EU P P' t1 s1 -> EU P P' t0 s0.
+| EU_step : P t0 s0 -> forall t1 s1, step t0 s0 t1 s1 -> EU P P' t1 s1 -> EU P P' t0 s0.
+Arguments EU_here {S R P P' t0 s0}.
+Arguments EU_step {S R P P' t0 s0}.
 
-Lemma eq_sat_EU {S1 S2 R1 R2} q (P1 P1' : TPred S1 R1) (P2 P2' : TPred S2 R2) :
-    eq_sat_sep_sbuter q P1 P2 -> eq_sat_sep_sbuter q P1' P2' ->
-    eq_sat_sep_sbuter q (EU P1 P1') (EU P2 P2').
+Lemma eq_sat_EU {S1 S2 R1 R2} q Q (P1 P1' : TPred S1 R1) (P2 P2' : TPred S2 R2) :
+    eq_sat_sep_sbuter q Q P1 P2 -> eq_sat_sep_sbuter q Q P1' P2' ->
+    eq_sat_sep_sbuter q Q (EU P1 P1') (EU P2 P2').
 Proof.
   intros eq_sat_Ps eq_sat_P's; split; intros.
   - revert p t2 s2 H H0 H1 H2; dependent induction H3; intros.
@@ -164,11 +166,15 @@ Qed.
 
 (** * `eq_sat_sep_sbuter` for `EF`  **)
 
-Definition EF {S R} := @EU S R (fun _ _ => True).
+Notation True2 := (fun _ _ => True).
 
-Lemma eq_sat_EF {S1 S2 R1 R2} q (P1 : TPred S1 R1) (P2 : TPred S2 R2) :
-    eq_sat_sep_sbuter q P1 P2 ->
-    eq_sat_sep_sbuter q (EF P1) (EF P2).
+Notation EF := (EU True2).
+Notation EF_here := (@EU_here _ _ True2 _ _ _).
+Notation EF_step := (@EU_step _ _ True2 _ _ _ I).
+
+Lemma eq_sat_EF {S1 S2 R1 R2} q Q (P1 : TPred S1 R1) (P2 : TPred S2 R2) :
+    eq_sat_sep_sbuter q Q P1 P2 ->
+    eq_sat_sep_sbuter q Q (EF P1) (EF P2).
 Proof. eapply eq_sat_EU; easy. Qed.
 
 
@@ -183,9 +189,9 @@ Lemma is_path_gen_mon {S R P} : monotone2 (@AG_gen S R P).
 Proof. repeat intro; induction IN; econstructor; eauto. Qed.
 Hint Resolve is_path_gen_mon : paco.
 
-Lemma eq_sat_AG {S1 S2 R1 R2} q (P1 : TPred S1 R1) (P2 : TPred S2 R2) :
-    eq_sat_sep_sbuter q P1 P2 ->
-    eq_sat_sep_sbuter q (AG P1) (AG P2).
+Lemma eq_sat_AG {S1 S2 R1 R2} q Q (P1 : TPred S1 R1) (P2 : TPred S2 R2) :
+    eq_sat_sep_sbuter q Q P1 P2 ->
+    eq_sat_sep_sbuter q Q (AG P1) (AG P2).
 Proof.
   intros eq_sat_Ps; split; intros.
   - revert p t1 s1 t2 s2 H H0 H1 H2 H3; pcofix CIH; intros.
@@ -239,10 +245,12 @@ Inductive AU {S R} (P P' : TPred S R) t0 s0 : Prop :=
 | AU_step : P t0 s0 -> steps t0 s0 ->
             (forall t1 s1, step t0 s0 t1 s1 -> AU P P' t1 s1) ->
             AU P P' t0 s0.
+Arguments AU_here {S R P P' t0 s0}.
+Arguments AU_step {S R P P' t0 s0}.
 
-Lemma eq_sat_AU {S1 S2 R1 R2} q (P1 P1' : TPred S1 R1) (P2 P2' : TPred S2 R2) :
-    eq_sat_sep_sbuter q P1 P2 -> eq_sat_sep_sbuter q P1' P2' ->
-    eq_sat_sep_sbuter q (AU P1 P1') (AU P2 P2').
+Lemma eq_sat_AU {S1 S2 R1 R2} q Q (P1 P1' : TPred S1 R1) (P2 P2' : TPred S2 R2) :
+    eq_sat_sep_sbuter q Q P1 P2 -> eq_sat_sep_sbuter q Q P1' P2' ->
+    eq_sat_sep_sbuter q Q (AU P1 P1') (AU P2 P2').
 Proof.
   intros eq_sat_Ps eq_sat_P's; split; intros.
   - revert p t2 s2 H H0 H1 H2; dependent induction H3; intros.
@@ -296,11 +304,13 @@ Qed.
 
 (** * `eq_sat_sep_sbuter` for `AF` **)
 
-Definition AF {S R} := @AU S R (fun _ _ => True).
+Notation AF := (AU True2).
+Notation AF_here := (@AU_here _ _ True2 _ _ _).
+Notation AF_step := (@AU_step _ _ True2 _ _ _ I).
 
-Lemma eq_sat_AF {S1 S2 R1 R2} q (P1 : TPred S1 R1) (P2 : TPred S2 R2) :
-    eq_sat_sep_sbuter q P1 P2 ->
-    eq_sat_sep_sbuter q (AF P1) (AF P2).
+Lemma eq_sat_AF {S1 S2 R1 R2} q Q (P1 : TPred S1 R1) (P2 : TPred S2 R2) :
+    eq_sat_sep_sbuter q Q P1 P2 ->
+    eq_sat_sep_sbuter q Q (AF P1) (AF P2).
 Proof. apply eq_sat_AU; easy. Qed.
 
 
@@ -321,9 +331,9 @@ Hint Resolve EG_gen_mon : paco.
 Definition EG_pf {S R P t0 s0} : @EG S R P t0 s0 -> P t0 s0.
 Proof. intro; punfold H; destruct H; eauto. Defined.
 
-Lemma eq_sat_EG {S1 S2 R1 R2} q (P1 : TPred S1 R1) (P2 : TPred S2 R2) :
-    eq_sat_sep_sbuter q P1 P2 ->
-    eq_sat_sep_sbuter q (EG P1) (EG P2).
+Lemma eq_sat_EG {S1 S2 R1 R2} q Q (P1 : TPred S1 R1) (P2 : TPred S2 R2) :
+    eq_sat_sep_sbuter q Q P1 P2 ->
+    eq_sat_sep_sbuter q Q (EG P1) (EG P2).
 Proof.
   intro eq_sat_Ps; split; intros.
   - revert p t1 s1 t2 s2 H H0 H1 H2 H3; pcofix CIH; intros.
@@ -387,9 +397,142 @@ Proof.
 Qed.
 
 
+(** * `eq_sat_sep_sbuter` for termination predicates **)
+
+Definition RetPred S R := R -> S -> Prop.
+
+Definition AReturns {S R} (P : RetPred S R) : TPred S R :=
+  AF (fun t s => exists r, observing eq (Ret r) t /\ P r s).
+
+Definition eq_sat_sep_ret {S1 S2 R1 R2} q Q
+  (P1 : RetPred S1 R1) (P2 : RetPred S2 R2) :=
+  forall p r1 r2 s1 s2, pre q (s1,s2) -> p ⊥ q ->
+    p ∈ Q r1 r2 -> (P1 r1 s1 <-> P2 r2 s2).
+
+Lemma eq_sat_AReturns {S1 S2 R1 R2} q Q (P1 : RetPred S1 R1) (P2 : RetPred S2 R2) :
+  eq_sat_sep_ret q Q P1 P2 ->
+  eq_sat_sep_sbuter q Q (AReturns P1) (AReturns P2).
+Proof.
+  intro eq_sat_Ps; unfold AReturns; split; intros.
+  - revert p t2 s2 H H0 H1 H2; dependent induction H3; intros.
+    + destruct H as [? [[]]].
+      punfold H2; red in H2; destruct H.
+      dependent induction H2; try solve [ inv H7 ].
+      * eapply AF_here; exists r2; split; eauto.
+        eapply (eq_sat_Ps p'); eauto.
+      * punfold H3; red in H3; destruct x; inv H3.
+      * eapply AF_step; eauto; intros.
+        eapply H5; eauto.
+        -- respects; eapply sep_r; eauto.
+        -- eapply step_no_errors; eauto.
+    + punfold H5; red in H5; dependent induction H5.
+      * red in H0; destruct x0; inv H0.
+      * punfold H5; red in H5; destruct x; inv H5.
+      * destruct (stepsF_impl_stepF _ _ H8) as [?t1' [?s1' []]].
+        eapply (H2 _ _ X p'); eauto.
+        -- respects; eapply sep_r; eauto.
+        -- pfold; red; eapply H10; eauto.
+      * apply AF_step; eauto; intros.
+        eapply H5; eauto.
+        -- respects; eapply sep_r; eauto.
+        -- eapply step_no_errors; eauto.
+      * apply AF_step; eauto; intros.
+        specialize (H5 _ _ X); destruct H5 as [?t1' [?s1' [? []]]].
+        eapply (H2 _ _ x p'); pclearbot; eauto.
+        -- respects; eapply sep_r; eauto.
+        -- eapply step_no_errors; eauto.
+  - revert p t1 s1 H H0 H1 H2; dependent induction H3; intros.
+    + destruct H as [? [[]]].
+      punfold H2; red in H2; destruct H.
+      dependent induction H2; try solve [ inv H2 | inv H7 ].
+      * eapply AF_here; exists r1; split; eauto.
+        eapply (eq_sat_Ps p'); eauto.
+      * eapply AF_step; eauto; intros.
+        eapply H5; eauto.
+        respects; eapply sep_r; eauto.
+    + punfold H5; red in H5; dependent induction H5.
+      * red in H0; destruct x; inv H0.
+      * punfold H5; red in H5; destruct x; inv H5.
+      * apply AF_step; eauto; intros.
+        eapply H5; eauto.
+        respects; eapply sep_r; eauto.
+      * destruct (stepsF_impl_stepF _ _ H8) as [?t2' [?s2' []]].
+        eapply (H2 _ _ X p'); eauto.
+        -- respects; eapply sep_r; eauto.
+        -- pfold; red; eapply H10; eauto.
+        -- eapply step_no_errors; eauto.
+      * apply AF_step; eauto; intros.
+        specialize (H10 _ _ X); destruct H10 as [?t2' [?s2' [? []]]].
+        eapply (H2 _ _ x p'); pclearbot; eauto.
+        -- respects; eapply sep_r; eauto.
+        -- eapply step_no_errors; eauto.
+Qed.
+
+Definition EReturns {S R} (P : RetPred S R) : TPred S R :=
+  EF (fun t s => exists r, observing eq (Ret r) t /\ P r s).
+
+Lemma eq_sat_EReturns {S1 S2 R1 R2} q Q (P1 : RetPred S1 R1) (P2 : RetPred S2 R2) :
+  eq_sat_sep_ret q Q P1 P2 ->
+  eq_sat_sep_sbuter q Q (EReturns P1) (EReturns P2).
+Proof.
+  intros eq_sat_Ps; unfold EReturns; split; intros.
+  - revert p t2 s2 H H0 H1 H2; dependent induction H3; intros.
+    + destruct H as [r1 []]; eapply Proper_observing_sbuter in H2; eauto.
+      punfold H2; red in H2; dependent induction H2; try solve [ inv H8 ].
+      * eapply EF_here; exists r2; split; eauto.
+        eapply (eq_sat_Ps p'); eauto.
+      * punfold H3; red in H3; destruct x; inv H3.
+      * destruct (stepsF_impl_stepF _ _ H8) as [?t2' [?s2' []]].
+        eapply EF_step; eauto.
+        eapply H6; eauto.
+        -- respects; eapply sep_r; eauto.
+        -- eapply step_no_errors; eauto.
+    + punfold H2; red in X, H2; dependent induction H2.
+      * destruct x0; inv X.
+      * punfold H4; red in H4; destruct x; inv H4.
+      * eapply (IHEU p'); eauto.
+        -- respects; eapply sep_r; eauto.
+        -- pfold; red; eapply H4; eauto.
+      * destruct (stepsF_impl_stepF _ _ H2) as [?t2' [?s2' []]].
+        eapply EF_step; eauto.
+        eapply H5; eauto.
+        -- respects; eapply sep_r; eauto.
+        -- eapply step_no_errors; eauto.
+      * destruct (H4 _ _ X) as [?t2' [?s2' [? []]]].
+        eapply EF_step; eauto.
+        eapply (IHEU p'); pclearbot; eauto.
+        -- respects; eapply sep_r; eauto.
+        -- eapply step_no_errors; eauto.
+  - revert p t1 s1 H H0 H1 H2; dependent induction H3; intros.
+    + destruct H as [r2 []]; eapply Proper_observing_sbuter in H2; eauto.
+      punfold H2; red in H2; dependent induction H2; try solve [ inv H2 | inv H8 ].
+      * eapply EF_here; exists r1; split; eauto.
+        eapply (eq_sat_Ps p'); eauto.
+      * destruct (stepsF_impl_stepF _ _ H8) as [?t2' [?s2' []]].
+        eapply EF_step; eauto.
+        eapply H6; eauto.
+        respects; eapply sep_r; eauto.
+    + punfold H2; red in X, H2; dependent induction H2.
+      1-2: destruct x; inv X.
+      * destruct (stepsF_impl_stepF _ _ H2) as [?t1' [?s1' []]].
+        eapply EF_step; eauto.
+        eapply H5; eauto.
+        respects; eapply sep_r; eauto.
+      * eapply (IHEU p'); eauto.
+        -- respects; eapply sep_r; eauto.
+        -- pfold; red; eapply H4; eauto.
+        -- eapply step_no_errors; eauto.
+      * destruct (H5 _ _ X) as [?t1' [?s1' [? []]]].
+        eapply EF_step; eauto.
+        eapply (IHEU p'); pclearbot; eauto.
+        -- respects; eapply sep_r; eauto.
+        -- eapply step_no_errors; eauto.
+Qed.
+
+
 (** * Definition of our fragment of CTL **)
 
-Inductive CTLformula {S} : Type :=
+Inductive CTLformula {S R} : Type :=
 | CTL_st (P:S -> Prop)
 | CTL_and (tp1 tp2:CTLformula)
 | CTL_or (tp1 tp2:CTLformula)
@@ -399,9 +542,11 @@ Inductive CTLformula {S} : Type :=
 | CTL_AF (tp:CTLformula)
 | CTL_AG (tp:CTLformula)
 | CTL_EU (tp1 tp1:CTLformula)
-| CTL_AU (tp1 tp1:CTLformula).
+| CTL_AU (tp1 tp1:CTLformula)
+| CTL_EReturns (P : RetPred S R)
+| CTL_AReturns (P : RetPred S R).
 
-Fixpoint CTLsats {S R} (tp:@CTLformula S): TPred S R :=
+Fixpoint CTLsats {S R} (tp:@CTLformula S R): TPred S R :=
   match tp with
   | CTL_st P => state_pred _ P
   | CTL_and tp1 tp2 => (CTLsats tp1) /2\ (CTLsats tp2)
@@ -413,28 +558,34 @@ Fixpoint CTLsats {S R} (tp:@CTLformula S): TPred S R :=
   | CTL_AG tp => AG (CTLsats tp)
   | CTL_EU tp1 tp2 => EU (CTLsats tp1) (CTLsats tp2)
   | CTL_AU tp1 tp2 => AU (CTLsats tp1) (CTLsats tp2)
+  | CTL_EReturns P => EReturns P
+  | CTL_AReturns P => AReturns P
   end.
 
-Inductive CTLsim {S1 S2} q: @CTLformula S1 -> @CTLformula S2 -> Prop :=
-| CTLsim_st P1 P2 : q_similar q P1 P2 -> CTLsim q (CTL_st P1) (CTL_st P2)
-| CTLsim_and tp1 tp2 tp1' tp2' : CTLsim q tp1 tp2 -> CTLsim q tp1' tp2' ->
-                                CTLsim q (CTL_and tp1 tp1') (CTL_and tp2 tp2')
-| CTLsim_or tp1 tp2 tp1' tp2' : CTLsim q tp1 tp2 -> CTLsim q tp1' tp2' ->
-                               CTLsim q (CTL_or tp1 tp1') (CTL_or tp2 tp2')
-| CTLsim_impl tp1 tp2 tp1' tp2' : CTLsim q tp1 tp2 -> CTLsim q tp1' tp2' ->
-                                 CTLsim q (CTL_impl tp1 tp1') (CTL_impl tp2 tp2')
-| CTLsim_EF tp1 tp2 : CTLsim q tp1 tp2 -> CTLsim q (CTL_EF tp1) (CTL_EF tp2)
-| CTLsim_EG tp1 tp2 : CTLsim q tp1 tp2 -> CTLsim q (CTL_EG tp1) (CTL_EG tp2)
-| CTLsim_AF tp1 tp2 : CTLsim q tp1 tp2 -> CTLsim q (CTL_AF tp1) (CTL_AF tp2)
-| CTLsim_AG tp1 tp2 : CTLsim q tp1 tp2 -> CTLsim q (CTL_AG tp1) (CTL_AG tp2)
-| CTLsim_EU tp1 tp2 tp1' tp2' : CTLsim q tp1 tp2 -> CTLsim q tp1' tp2' ->
-                               CTLsim q (CTL_EU tp1 tp1') (CTL_EU tp2 tp2')
-| CTLsim_AU tp1 tp2 tp1' tp2' : CTLsim q tp1 tp2 -> CTLsim q tp1' tp2' ->
-                               CTLsim q (CTL_AU tp1 tp1') (CTL_AU tp2 tp2')
+Inductive CTLsim {S1 S2 R1 R2} q Q: @CTLformula S1 R1 -> @CTLformula S2 R2 -> Prop :=
+| CTLsim_st P1 P2 : q_similar q P1 P2 -> CTLsim q Q (CTL_st P1) (CTL_st P2)
+| CTLsim_and tp1 tp2 tp1' tp2' : CTLsim q Q tp1 tp2 -> CTLsim q Q tp1' tp2' ->
+                                CTLsim q Q (CTL_and tp1 tp1') (CTL_and tp2 tp2')
+| CTLsim_or tp1 tp2 tp1' tp2' : CTLsim q Q tp1 tp2 -> CTLsim q Q tp1' tp2' ->
+                               CTLsim q Q (CTL_or tp1 tp1') (CTL_or tp2 tp2')
+| CTLsim_impl tp1 tp2 tp1' tp2' : CTLsim q Q tp1 tp2 -> CTLsim q Q tp1' tp2' ->
+                                 CTLsim q Q (CTL_impl tp1 tp1') (CTL_impl tp2 tp2')
+| CTLsim_EF tp1 tp2 : CTLsim q Q tp1 tp2 -> CTLsim q Q (CTL_EF tp1) (CTL_EF tp2)
+| CTLsim_EG tp1 tp2 : CTLsim q Q tp1 tp2 -> CTLsim q Q (CTL_EG tp1) (CTL_EG tp2)
+| CTLsim_AF tp1 tp2 : CTLsim q Q tp1 tp2 -> CTLsim q Q (CTL_AF tp1) (CTL_AF tp2)
+| CTLsim_AG tp1 tp2 : CTLsim q Q tp1 tp2 -> CTLsim q Q (CTL_AG tp1) (CTL_AG tp2)
+| CTLsim_EU tp1 tp2 tp1' tp2' : CTLsim q Q tp1 tp2 -> CTLsim q Q tp1' tp2' ->
+                               CTLsim q Q (CTL_EU tp1 tp1') (CTL_EU tp2 tp2')
+| CTLsim_AU tp1 tp2 tp1' tp2' : CTLsim q Q tp1 tp2 -> CTLsim q Q tp1' tp2' ->
+                               CTLsim q Q (CTL_AU tp1 tp1') (CTL_AU tp2 tp2')
+| CTLsim_EReturns P1 P2 : eq_sat_sep_ret q Q P1 P2 ->
+                         CTLsim q Q (CTL_EReturns P1) (CTL_EReturns P2)
+| CTLsim_AReturns P1 P2 : eq_sat_sep_ret q Q P1 P2 ->
+                         CTLsim q Q (CTL_AReturns P1) (CTL_AReturns P2)
 .
 
-Lemma tpsim_implies_eq_sat_sep_sbuter {S1 S2 R1 R2} q TP1 TP2:
-  CTLsim q TP1 TP2 -> @eq_sat_sep_sbuter S1 S2 R1 R2 q (CTLsats TP1) (CTLsats TP2).
+Lemma tpsim_implies_eq_sat_sep_sbuter {S1 S2 R1 R2} q Q TP1 TP2:
+  CTLsim q Q TP1 TP2 -> @eq_sat_sep_sbuter S1 S2 R1 R2 q Q (CTLsats TP1) (CTLsats TP2).
 Proof.
   intro tp_sim; induction tp_sim.
   - apply eq_sat_state_preds; eauto.
@@ -447,13 +598,15 @@ Proof.
   - apply eq_sat_AG; eauto.
   - apply eq_sat_EU; eauto.
   - apply eq_sat_AU; eauto.
+  - apply eq_sat_EReturns; eauto.
+  - apply eq_sat_AReturns; eauto.
 Qed.
 
 Theorem sbuter_preserves_tpreds {S1 R1 S2 R2} p q Q t1 s1 t2 s2 TP1 TP2:
   @sbuter S1 R1 S2 R2 p Q t1 s1 t2 s2 -> no_errors t2 s2 ->
-  CTLsim q TP1 TP2 -> pre (p ** q) (s1, s2) ->
+  CTLsim q Q TP1 TP2 -> pre (p ** q) (s1, s2) ->
   CTLsats TP1 t1 s1 <-> CTLsats TP2 t2 s2.
 Proof.
   intros sb ne tp_sim pre_pq. destruct pre_pq as [ pre_p [ pre_q sep ]].
-  eapply (tpsim_implies_eq_sat_sep_sbuter q TP1 TP2 tp_sim); eauto.
+  eapply (tpsim_implies_eq_sat_sep_sbuter q Q TP1 TP2 tp_sim); eauto.
 Qed.
